disk-betree/DiskBetree.dfy
@@ -1,16 +1,13 @@
-include "../lib/total_order.dfy"
 include "BlockCache.dfy"  
 include "../lib/sequences.dfy"
+include "MapSpec.dfy"
 
 abstract module DiskBetree {
+  import MS: MapSpec
   import BC : BlockCache
-  import K : Total_Order
   import opened Sequences
   
-  type Key = K.Element
-
-  // Users must provide a definition of EmptyValue
-  function EmptyValue<Value>() : Value
+  type Key = MS.Key
     
   datatype BufferEntry<Value> = Insertion(value: Value)
 
@@ -24,7 +21,7 @@ abstract module DiskBetree {
   predicate BufferIsDefining(log: seq<BufferEntry>) {
     && |log| > 0
   }
-  
+
   predicate BufferDefinesValue<Value>(log: seq<BufferEntry>, value: Value) {
     && BufferIsDefining(log)
     && log[0].value == value
@@ -39,9 +36,10 @@ abstract module DiskBetree {
     && |lookup| > 0
     && lookup[0].ref == BC.Root(k.bcc)
     && (forall i :: 0 <= i < |lookup| - 1 ==> key in lookup[i].node.children && lookup[i].node.children[key] == lookup[i+1].ref)
-    && (forall i :: 0 <= i < |lookup| ==> BC.Read(k.bcc, s.bcv, lookup[i].ref, lookup[i].node))
+    && (forall i :: 0 <= i < |lookup| ==> BC.Read(k.bcc, s.bcv, lookup[i].ref) == lookup[i].node)
     && (forall i :: 0 <= i < |lookup| ==> WFNode(lookup[i].node))
-    && (forall i :: 0 <= i < |lookup| ==> lookup[i].accumulatedBuffer == (if i > 0 then lookup[i-1].accumulatedBuffer else []) + lookup[i].node.buffer[key])
+    && lookup[0].accumulatedBuffer == lookup[0].node.buffer[key]
+    && (forall i :: 0 < i < |lookup| ==> lookup[i].accumulatedBuffer == lookup[i-1].accumulatedBuffer + lookup[i].node.buffer[key])
     && BufferDefinesValue(Last(lookup).accumulatedBuffer, value)
   }
 
@@ -55,23 +53,33 @@ abstract module DiskBetree {
   datatype Constants = Constants(bcc: BC.Constants)
   datatype Variables<Value> = Variables(bcv: BC.Variables<Node<Value>>)
 
+  function EmptyNode<Value>() : Node {
+    var buffer := imap key | MS.InDomain(key) :: [Insertion(MS.EmptyValue())];
+    Node(imap[], buffer)
+  }
+    
+  predicate Init(k: Constants, s: Variables) {
+    && BC.Init(k.bcc, s.bcv)
+    && BC.Read(k.bcc, s.bcv, BC.Root(k.bcc)) == EmptyNode()
+  }
+    
   predicate Query<Value>(k: Constants, s: Variables, s': Variables, key: Key, value: Value, lookup: Lookup) {
     && s == s'
     && IsSatisfyingLookup(k, s, key, value, lookup)
   }
 
   predicate InsertMessage<Value>(k: Constants, s: Variables, s': Variables, key: Key, value: Value, oldroot: Node) {
-    && BC.Read(k.bcc, s.bcv, BC.Root(k.bcc), oldroot)
+    && BC.Read(k.bcc, s.bcv, BC.Root(k.bcc)) == oldroot
     && WFNode(oldroot)
     && var newroot := Node(oldroot.children, oldroot.buffer[key := [Insertion(value)] + oldroot.buffer[key]]);
     && WFNode(oldroot)
     && BC.Apply(k.bcc, s.bcv, s'.bcv, BC.WriteOp(BC.Root(k.bcc), newroot, Successors(newroot)))
   }
 
-  predicate Flush<Value>(k: Constants, s: Variables, s': Variables, parentref: BC.Reference, parent: Node, childref: BC.Reference, child: Node, newchildref: BC.Reference, sint: BC.Variables) {
+  predicate Flush<Value>(k: Constants, s: Variables, s': Variables, parentref: BC.Reference, parent: Node, childref: BC.Reference, child: Node, newchildref: BC.Reference) {
     var movedKeys := iset k | k in parent.children && parent.children[k] == childref;
-    && BC.Read(k.bcc, s.bcv, parentref, parent)
-    && BC.Read(k.bcc, s.bcv, childref, child)
+    && BC.Read(k.bcc, s.bcv, parentref) == parent
+    && BC.Read(k.bcc, s.bcv, childref) == child
     && WFNode(parent)
     && WFNode(child)
     && var newbuffer := imap k :: (if k in movedKeys then parent.buffer[k] + child.buffer[k] else child.buffer[k]);
@@ -83,12 +91,31 @@ abstract module DiskBetree {
     && BC.Apply2(k.bcc, s.bcv, s'.bcv, allocop, writeop)
   }
 
-  predicate Grow(k: Constants, s: Variables, s': Variables, oldroot: Node, newchildref: BC.Reference, sint: BC.Variables) {
-    && BC.Read(k.bcc, s.bcv, BC.Root(k.bcc), oldroot)
+  predicate Grow(k: Constants, s: Variables, s': Variables, oldroot: Node, newchildref: BC.Reference) {
+    && BC.Read(k.bcc, s.bcv, BC.Root(k.bcc)) == oldroot
     && var newchild := oldroot;
-    && var newroot := Node(imap k :: newchildref, imap[]);
+    && var newroot := Node(imap key | MS.InDomain(key) :: newchildref, imap[]);
     && var allocop := BC.AllocOp(newchild, Successors(newchild), newchildref);
     && var writeop := BC.WriteOp(BC.Root(k.bcc), newroot, Successors(newroot));
     && BC.Apply2(k.bcc, s.bcv, s'.bcv, allocop, writeop)
+  }
+
+  datatype Step<Value(!new)> =
+    | QueryStep(key: Key, value: Value, lookup: Lookup)
+    | InsertMessageStep(key: Key, value: Value, oldroot: Node)
+    | FlushStep(parentref: BC.Reference, parent: Node, childref: BC.Reference, child: Node, newchildref: BC.Reference)
+    | GrowStep(oldroot: Node, newchildref: BC.Reference)
+
+  predicate NextStep(k: Constants, s: Variables, s': Variables, step: Step) {
+    match step {
+      case QueryStep(key, value, lookup) => Query(k, s, s', key, value, lookup)
+      case InsertMessageStep(key, value, oldroot) => InsertMessage(k, s, s', key, value, oldroot)
+      case FlushStep(parentref, parent, childref, child, newchildref) => Flush(k, s, s', parentref, parent, childref, child, newchildref)
+      case GrowStep(oldroot, newchildref) => Grow(k, s, s', oldroot, newchildref)
+    }
+  }
+
+  predicate Next<Value(!new)>(k: Constants, s: Variables, s': Variables) {
+    exists step: Step :: NextStep(k, s, s', step)
   }
 }
