disk-betree/MapSpec.dfy
@@ -1,0 +1,90 @@
+include "../tla-tree/MissingLibrary.dfy"
+include "../lib/total_order.dfy"
+
+abstract module MapSpec {
+import opened MissingLibrary
+
+import Keyspace : Total_Order
+type Key = Keyspace.Element
+
+
+// Users must provide a definition of EmptyValue
+function EmptyValue<Value>() : Value
+
+datatype Constants = Constants()
+type View<Value> = imap<Key, Value>
+datatype Variables<Value> = Variables(view:View<Value>)
+
+predicate ViewComplete(view:View)
+{
+    forall k :: k in view
+}
+
+predicate WF(s:Variables)
+{
+    && ViewComplete(s.view)
+}
+
+// Dafny black magic: This name is here to give EmptyMap's forall something to
+// trigger on. (Eliminates a /!\ Warning.)
+predicate InDomain(k:Key)
+{
+    true
+}
+
+function EmptyMap<Value>() : (zmap : imap<Key,Value>)
+    ensures ViewComplete(zmap)
+{
+    imap k | InDomain(k) :: EmptyValue()
+}
+
+predicate Init(k:Constants, s:Variables)
+    ensures Init(k, s) ==> WF(s)
+{
+    s == Variables(EmptyMap())
+}
+
+predicate Query<Value>(k:Constants, s:Variables, s':Variables, key:Key, result:Value)
+    requires WF(s)
+{
+    && result == s.view[key]
+    && s' == s
+}
+
+predicate Write<Value>(k:Constants, s:Variables, s':Variables, key:Key, new_value:Value)
+    requires WF(s)
+    ensures Write(k, s, s', key, new_value) ==> WF(s')
+{
+    && WF(s')
+    && s'.view == s.view[key := new_value]
+}
+
+predicate Stutter(k:Constants, s:Variables, s':Variables)
+    requires WF(s)
+{
+    s' == s
+}
+
+datatype Step<Value> =
+    | QueryStep(key:Key, result:Value)
+    | WriteStep(key:Key, new_value:Value)
+    | StutterStep
+
+predicate NextStep(k:Constants, s:Variables, s':Variables, step:Step)
+    requires WF(s)
+{
+    match step {
+        case QueryStep(key, result) => Query(k, s, s', key, result)
+        case WriteStep(key, new_value) => Write(k, s, s', key, new_value)
+        case StutterStep() => Stutter(k, s, s')
+    }
+}
+
+predicate Next<Value(!new)>(k:Constants, s:Variables, s':Variables)
+    requires WF(s)
+    ensures Next(k, s, s') ==> WF(s')
+{
+    exists step :: NextStep<Value>(k, s, s', step)
+}
+
+}
